Upd

SkipList2/SkipList.Remove.fst
@@ -1,138 +1,32 @@
-module SkipList2.Remove
-
-open SkipList2.Statement
-open SkipList2.Properties
-open SkipList2.Seq.Properties
-open FStar.Option
-open FStar.Seq
-open FStar.List.Tot
-
-module Sl = SkipList2.Statement
-module List = FStar.List.Tot
-module Seq = FStar.Seq
+module SkipList.Remove
 
 
-assume val lemma_more : #a: eqtype -> #f: cmp a -> sl: skipList a f {Sl.length sl > 0} -> 
-        Lemma(ensures(forall 
-            (counter_global : nat{counter_global < Sl.length sl}) 
-            (counter_local : nat {counter_local < List.length (getIndex sl counter_global)}) .
-            List.index (getIndex sl counter_global) counter_local > counter_global))
-
- val rebuildIndexesList:#a: eqtype -> #f : cmp a -> sl: skipList a f {Sl.length sl > 1} ->  
-                                 index: nat -> lst: non_empty_list nat
-                                    {forall (counter_local: nat {counter_local < List.length lst}).
-                                    List.index lst counter_local > index} ->
-                                lst_return : non_empty_list nat ->    
-                                counter: nat {counter < List.length lst} -> 
-                                lst_deleted: non_empty_list nat -> 
-                                 place: nat ->
-                                   ML(non_empty_list nat)
-
-let rec rebuildIndexesList #a #f sl index lst lst_return counter lst_deleted place = 
-    let hd = List.index lst counter in 
-    let header = 
-        if (hd < place) then hd 
-        else if (hd = place) then 
-            (if (List.length lst_deleted > counter) 
-                then  (List.index lst_deleted counter) 
-                else (Sl.length sl - 2)
-            )
-        else (hd -1) 
-    in 
-    let lst_return = SkipList2.Seq.Properties.upd lst_return counter header in 
-    if ((counter + 1) < List.length lst) 
-        then rebuildIndexesList #a #f sl index lst lst_return (counter +1) lst_deleted place
-    else lst_return                        
-
-val rebuildIndexesSeq: #a: eqtype -> #f: cmp a -> sl: skipList a f {Sl.length sl > 1} -> 
-            place : nat {place < Sl.length sl - 1} ->
-            new_indexes: seq (non_empty_list nat) {Seq.length new_indexes =  Sl.length sl - 1} -> 
-            counter: nat {counter < Sl.length sl} (* for the last - just copy*) -> 
-            ML(r: seq (non_empty_list nat) {Seq.length r = Sl.length sl - 1})
-
-let rec rebuildIndexesSeq #a #f sl place new_indexes counter = 
-            if (counter = place) then 
-                rebuildIndexesSeq #a #f sl place new_indexes (counter +1) (* just skip the element*)
-            else 
-                let indexes = getIndex sl counter in lemma_more #a #f sl;
-                let rebuilt_list = rebuildIndexesList #a #f sl counter indexes indexes 0 (getIndex sl place) place in
-                let index_for_update = if counter > place then (counter - 1) else counter in  
-                let new_indexes = Seq.upd new_indexes index_for_update rebuilt_list in
-                if ((counter +1) < Sl.length sl) then 
-                    rebuildIndexesSeq #a #f sl place new_indexes (counter +1) 
-                else new_indexes     
+(* last element is less than the next one*)
+val _change_values: #a: eqtype -> #f: cmp a -> s1: seq a {Seq.sorted f s /\ element = Seq.index_last} ->  s: seq a {Seq.sorted f s }-> index: nat {index > place /\ index < Seq.length s} -> 
+Tot (r: seq a {Seq.sorted f s }) 
+let _change_values #a #f s index = 
+	assert (f (Seq.index last ) (Seq.index s index)  );
+	let s1 = append_right s1 (Seq.index s index);
+	assert (Seq.sorted f s1)
 
 
-val rebuildIndexes: #a: eqtype -> #f: cmp a ->sl: skipList a f {Sl.length sl > 1} -> 
-            place : nat {place < Sl.length sl - 1} -> 
-            ML(r: seq (non_empty_list nat){ Seq.length r = Sl.length sl - 1})
 
-let rebuildIndexes #a #f sl place = 
-        let seq_replace = Seq.create (Sl.length sl - 1) [0] in 
-        rebuildIndexesSeq #a #f sl place seq_replace 0 
+val change_values: #a: eqtype -> #f: cmp a -> s: seq a {Seq.sorted  f s } -> Tot(r: seq a {Seq.sorted f r})
+let change_values #a #f s = 
+	_change_values #a #f s place
+	
+val change_value_current: #a : eqtype -> #f: cmp a -> a: element -> f: (a -> a) -> Tot(element: a)
+let change_value_current #a
 
-val concat: #a: eqtype ->#f: cmp a ->  s1 : seq a {Seq.sorted f s1 } -> s2: seq a {Seq.sorted f s2 /\
-(Seq.length s1 > 0 /\ Seq.length s2 > 0 /\ f (seqLast s1) (seqFirst s2))} -> 
-    Tot(s3: seq a {Seq.sorted f s3 /\ Seq.length s3 = Seq.length s1 + Seq.length s2})
+val _change_indexes_seq: #a: eqtype -> #f : cmp a -> s: seq a -> counter_global : nat {counter_global < Seq.length s} -> 
+	Tot(r: seq a {Seq.length s = Seq.length r + 1})
 
-let concat #a #f s1 s2 = 
-        let pivot = seqFirst s2 in 
-        let seq2 = Seq.tail s2 in 
-        assert(f (seqLast s1) pivot);
-        if (Seq.length seq2 = 0 ) then 
-            ordered_addition_l #a #f pivot s1
-        else (
-            tail_mem_left_wrapper #a #f pivot seq2; 
-            assert(forall y. (Seq.mem y seq2 ==> f pivot y));
-            assert(Seq.sorted f seq2);
-            tail_mem #a #f pivot s1; 
-            assert(forall y. (Seq.mem y s1 ==> f y pivot));
-            let r = sorted_seq_concat_wrapper #a #f pivot s1 seq2 
-            in r
-        )
+let _change_indexes_seq : #a: eqtype -> #f: cmp a -> s: seq a -> counter_local : nat {counter_local < List.length (getIndex s counter_global)} -> 
+	let 
 
+val change_indexes: #a: eqtype -> #f : cmp a -> s: seq a -> Tot(r: seq a {Seq.length s = Seq.length r + 1})
+let change_indexes #a #f s = 
+		
 
-assume val lemma_split: #a : eqtype -> #f: cmp a-> 
-            s: seq a {Seq.length s > 0 /\ Seq.sorted f s} ->
-                                place : nat {place <= Seq.length s} -> 
-                                Lemma (ensures 
-                                    ( 
-                                        (Seq.sorted f (fst(Seq.split s place))) /\ 
-                                        (Seq.sorted f (snd(Seq.split s place)))
-                                ))
-
-assume val lemma_sorted : #a: eqtype -> #f : cmp a -> s: seq a {Seq.sorted f s} ->
-            place : nat {place > 0 /\ place < Seq.length s -1 } -> 
-            Lemma (ensures (f (Seq.index s (place -1)) (Seq.index s place)))
-
-val rebuildSequence: #a: eqtype ->  #f: cmp a -> s:seq a{Seq.sorted f s /\ Seq.length s > 1 } ->  
-                place: nat {place < Seq.length s - 1} ->
-                Tot (r: seq a {Seq.sorted f r /\ Seq.length r = Seq.length s - 1})
-
-
-let rebuildSequence #a #f s place = 
-    let s1, s2 = Seq.split s place in (*place < Seq.length s -1  - it means that there is at least ONE element in right seq*)
-    lemma_split #a #f s place;
-    let s3, s4 = Seq.split s2 1 in(* s3 has one element, while s4 could not have any*)
-    lemma_split #a #f s2 1;
-    if Seq.length s1 = 0 then s4
-    else if (Seq.length s4 = 0) then s1
-    else
-        (
-            lemma_sorted #a #f s place; 
-            assert(f (Seq.index s (place -1)) (Seq.index s (place)));
-            assert(f (seqLast s1) (seqFirst s4));    
-            concat #a #f s1 s4
-        )        
-
-val remove: #a: eqtype -> #f : cmp a -> 
-        sl: skipList a f {Sl.length sl > 1} -> 
-        place : nat {place < Sl.length sl - 1} ->
-        ML(r: skipList a f {Sl.length sl = Sl.length r + 1})
-
-let remove #a #f sl place = 
-    let values = Sl.getValues sl in 
-    let indexes = Sl.getIndexes sl in 
-    let values_new = rebuildSequence #a #f values place in 
-    let indexes_new = rebuildIndexes #a #f sl place in 
-    Sl.Mk #a #f values_new indexes_new 
+val change: #a: eqtype -> #f: cmp a -> sl: skipList a f {Sl.length sl > 1} -> Tot(r: skipList a f {Sl.length sl= Sl.length r + 1 })
+let change 
